---
layout: page
title: Reductio ad absurdum
nav_order: 4
has_children: false
has_toc: false
parent: Propositional logic 
grand_parent: Notes
---

## Proof by contradiction 

Suppose I can establish an absurdity by assuming the negation of something. 
What does this give us? Well, given $\neg A \vdash \bot$, we can prove 
$\neg \neg A$.

If we that the sun is not not up, that usually means that it is actually 
up, right? 

More formally, we want to know about jutisfying 
$$
\neg \neg A \vdash A
$$
Can this be done using the rules so far?

Unfortunately, **nothing** in our rules so far will allow us establish this. 
Adding this rule to our existing system yields some very useful conclusions. 

For example, given $\neg A \vdash \bot$, we already knew we could establish 
$\vdash \neg \neg A$ but now we also have $\vdash A$. 

The process of establishing $A$ by assuming $A$ doesn't hold and arguing to a
contradiction goes by the *Reductio ad absurdum* (RAA) or *proof by contradiction*. 

Another well-known conclusion is the *Law of the Excluded Middle* which is 
just 
$$
A \lor \neg A
$$
In other words, no matter what $A$ is either $A$ holds or it is doesn't. 

You might take a moment and think this an immutable law of reality. 
Our day-to-day experience definitely leads us to think this. But reality in 
general is more complicated. Think of [Schrodinger's
cat](https://en.wikipedia.org/wiki/Schr√∂dinger%27s_cat). Is the cat alive or 
not alive in the box? What is the state of the unobserved wave function? 

But in an idealized world proof by contradiction is a perfectly reasonable 
assumption. And mathematicians, for the most part, tend to idealize our 
world. 

Below is a proof the Law of Excluded Middle using proof by contradiction.

{% eqn RAA_to_LEM %}
\begin{prooftree}
\infer0[\normalsize 1]{\neg(A \lor \neg A)} 
\infer0[\normalsize 1]{\neg(A \lor \neg A)}
\infer0[\normalsize 0]{A}
\infer2[\normalsize $\neg$ E]{\bot}
\infer1[\normalsize 0 $\neg$ I]{\neg A}
\infer1[\normalsize $\lor$ I${}_r$]{A \lor \neg A}
\infer2[\normalsize 1 $\neg$ E]{\bot}
\infer1[\normalsize RAA]{A \lor \neg A}
\end{prooftree}
{% endeqn %}

Given an formula of the form $A \to B$, the _contrapositive_ is the formula 
$$
\neg B \to \neg A
$$

Let's justify 
$$
A \to B \vdash \neg B \to \neg A 
$$

Below is a natural deduction proof
{% eqn Implies_contrapositive %}
\begin{prooftree}
\hypo{A \to B}
\infer0[\normalsize 0]{A}
\infer2{B}
\infer0[\normalsize 1]{\neg B}
\infer2{\bot}
\infer1[\normalsize 0]{\neg A}
\infer1[\normalsize 1]{\neg B \to \neg A}
\end{prooftree}
{% endeqn %}

If we substitute $\neg B$ for $A$ and $\neg A$ for $B$, we immediately have 
$$
\neg B \to \neg A \vdash (\neg \neg A) \to (\neg \neg B)
$$
With proof by contradiction, we get
$$
\neg B \to \neg A \vdash A \to B
$$

Establishing the contrapositive and deducing the original statement is 
uncommonly common pattern in mathematical argument.  
